print hashes

backend/Profilingaux.ml
@@ -1,8 +1,20 @@
 open Camlcoq
 open RTL
    
-let function_id (f : coq_function) : Z.t =
-  Z.of_uint 0;;
+let function_id (f : coq_function) : Digest.t =
+  Digest.string (Marshal.to_string f []);;
 
-let branch_id (f_id : Z.t) (node : P.t) =
-  Z.of_uint 0;;
+let branch_id (f_id : Digest.t) (node : P.t) : Digest.t =
+  Digest.string (f_id ^ (Int64.to_string (P.to_int64 node)));;
+
+let pp_id channel (x : Digest.t) =
+  for i=0 to 15 do
+    Printf.fprintf channel "%02x" (Char.code (String.get x i))
+  done
+
+let spp_id () (x : Digest.t) : string =
+  let s = ref "" in
+  for i=0 to 15 do
+    s := Printf.sprintf "%02x%s" (Char.code (String.get x i)) !s
+  done;
+  !s;;
