common/PrintAST.ml
@@ -63,7 +63,7 @@ let name_of_external = function
   | EF_debug(kind, text, targs) ->
      sprintf "debug%d %S" (P.to_int kind) (extern_atom text)
   | EF_profiling(id, kind) ->
-     sprintf "profiling %LX %d" (Z.to_int64 id) (Z.to_int kind)
+     sprintf "profiling %a %d" Profilingaux.spp_id id (Z.to_int kind)
 
 let rec print_builtin_arg px oc = function
   | BA x -> px oc x
